LeanSAT/Reflect/BVExpr/BitBlast/Lemmas/Sub.lean
@@ -1,0 +1,34 @@
+import LeanSAT.Reflect.BVExpr.BitBlast.Lemmas.Basic
+import LeanSAT.Reflect.BVExpr.BitBlast.Lemmas.Neg
+import LeanSAT.Reflect.BVExpr.BitBlast.Lemmas.Add
+import LeanSAT.Reflect.BVExpr.BitBlast.Impl.Sub
+
+open AIG
+
+namespace BVExpr
+namespace bitblast
+
+theorem blastSub_eq_eval_getLsb (aig : AIG BVBit) (lhs rhs : BVExpr w) (assign : Assignment)
+      (input : BinaryRefStream aig w)
+      (hleft : ∀ (idx : Nat) (hidx : idx < w), ⟦aig, input.lhs.getRef idx hidx, assign.toAIGAssignment⟧ = (lhs.eval assign).getLsb idx)
+      (hright : ∀ (idx : Nat) (hidx : idx < w), ⟦aig, input.rhs.getRef idx hidx, assign.toAIGAssignment⟧ = (rhs.eval assign).getLsb idx)
+    : ∀ (idx : Nat) (hidx : idx < w),
+        ⟦(blastSub aig input).aig, (blastSub aig input).stream.getRef idx hidx, assign.toAIGAssignment⟧
+          =
+        (lhs.eval assign - rhs.eval assign).getLsb idx := by
+  intros idx hidx
+  unfold blastSub
+  dsimp
+  rw [blastAdd_eq_eval_getLsb (lhs := lhs) (rhs := .un .neg rhs)]
+  . simp [BitVec.sub_toAdd]
+  . intro idx hidx
+    rw [AIG.LawfulStreamOperator.denote_mem_prefix]
+    . simp [hleft]
+    . simp [Ref.hgate]
+  . intro idx hidx
+    rw [blastNeg_eq_eval_getLsb (sub := rhs)]
+    . simp [BitVec.neg_eq_not_add]
+    . simp [hright]
+
+end bitblast
+end BVExpr
